src/dafny/test.dfy
@@ -1,0 +1,25 @@
+include "evm.dfy"
+
+import opened Int
+import opened EVM
+
+// Check most simple program possible
+method test_01() {
+  // Initialise SVM
+  var vm := create(map[],[PUSH1,0x80]);
+  // Execute program
+  vm := unwrap(execute(vm));
+  // Check what we know
+  assert operands(vm) == 1;
+  assert vm.pc == 2;
+  assert peek(vm,0) == 0x80;
+}
+
+/**
+ * Unwrap an EVM result on the assumption that it should be OK
+ * (i.e. not a REVERT or similar).
+ */
+function method unwrap(r:EVM.Result) : EVM.T
+  requires r.OK?{
+  var OK(v) := r; v
+}
